generational/spec/GC.Gen.CheneyGraphReadiness.fst
@@ -3789,6 +3789,85 @@ let chunked_cheney_collect_then_major_gc_live_subgraph_from_pre_gray_static_raw_
   chunked_cheney_collect_then_major_gc_live_subgraph_from_static_raw_target_policy
     minor major fp roots alloc_fuel fresh major_roots cap mark_fuel
 
+let chunked_cheney_collect_then_major_gc_live_subgraph_from_pre_gray_nonblue_static_raw_target_policy
+  (minor: minor_state) (major: MH.major_heap) (fp: U64.t)
+  (roots: seq U64.t) (alloc_fuel: nat) (fresh: MH.heap_chunk)
+  (major_roots: seq obj_addr)
+  (cap: nat{cap > 0})
+  (mark_fuel: nat)
+  : Lemma
+    (requires
+      minor_wf minor /\
+      alloc_fuel > 1 /\
+      GenInv.chunked_collection_heap_shape minor major fp alloc_fuel /\
+      SpecMajorAlloc.major_fl_chain_terminates major fp alloc_fuel = true /\
+      GenInv.chunked_chain_objects_blue major fp alloc_fuel /\
+      chunked_minor_preflight_value_policy minor major fp roots fresh /\
+      (let r =
+       SpecMajorAlloc.ensure_major_head_capacity_spec
+        major fp alloc_fuel
+        (PromotionDemand.minor_promotion_demand minor + 1)
+        fresh in
+       let collect =
+       ChunkedCheney.chunked_cheney_collect_spec
+        minor r.capacity_major_out r.capacity_fp_out roots
+        r.capacity_fuel_out in
+       GenInv.chunked_collection_heap_shape
+        collect.cmc_minor collect.cmc_major collect.cmc_fp
+        r.capacity_fuel_out /\
+       GenMajorGCBridge.chunked_major_roots_nonblue
+        collect.cmc_major major_roots /\
+       GenMajorGCBridge.chunked_major_edge_gen_field_witness
+        collect.cmc_major /\
+       GenMajorGCBridge.chunked_major_field_targets_non_infix
+        collect.cmc_major /\
+       ChunkedMarkTargetMembership.chunked_nonblue_scanned_raw_targets_in_major
+        collect.cmc_major /\
+       Seq.length (MH.major_objects collect.cmc_major) <= cap /\
+       mark_fuel > 0 /\
+       mark_fuel >= Seq.length (MH.major_objects collect.cmc_major)))
+    (ensures
+      chunked_cheney_collect_after_minor_promotion_head_preflight_post
+       minor major fp roots alloc_fuel fresh /\
+      (let r =
+       SpecMajorAlloc.ensure_major_head_capacity_spec
+        major fp alloc_fuel
+        (PromotionDemand.minor_promotion_demand minor + 1)
+        fresh in
+       let collect =
+       ChunkedCheney.chunked_cheney_collect_spec
+        minor r.capacity_major_out r.capacity_fp_out roots
+        r.capacity_fuel_out in
+       let (major_final, fp_final) =
+       ChunkedMajorGC.chunked_major_gc_bounded
+        (ChunkedMajorGCRoots.chunked_gray_roots
+          collect.cmc_major major_roots)
+        cap mark_fuel in
+       ChunkedMajorGCGraph.chunked_major_live_subgraph_preserved
+        collect.cmc_major major_final
+        (ChunkedMajorGCCorr.chunked_major_initial_reachable_live
+         collect.cmc_major major_roots)))
+  =
+  let r =
+    SpecMajorAlloc.ensure_major_head_capacity_spec
+      major fp alloc_fuel
+      (PromotionDemand.minor_promotion_demand minor + 1)
+      fresh in
+  let collect =
+    ChunkedCheney.chunked_cheney_collect_spec
+      minor r.capacity_major_out r.capacity_fp_out roots
+      r.capacity_fuel_out in
+  GenInv.chunked_collection_heap_shape_elim
+    collect.cmc_minor collect.cmc_major collect.cmc_fp r.capacity_fuel_out;
+  GenInv.chunked_major_alloc_shape_elim
+    collect.cmc_major collect.cmc_fp r.capacity_fuel_out;
+  GenMajorGCBridge.chunked_major_gc_bounded_after_gray_roots_nonblue_static_raw_target_policy_from_pre_gray
+    collect.cmc_major major_roots cap mark_fuel;
+  GenMajorGCBridge.chunked_major_gc_bounded_after_gray_roots_target_membership_policy_from_nonblue_static_raw_targets
+    collect.cmc_major major_roots cap mark_fuel;
+  chunked_cheney_collect_then_major_gc_live_subgraph_from_target_membership_policy
+    minor major fp roots alloc_fuel fresh major_roots cap mark_fuel
+
 let chunked_cheney_collect_then_major_gc_live_subgraph_from_raw_field_target_policy
   (minor: minor_state) (major: MH.major_heap) (fp: U64.t)
   (roots: seq U64.t) (alloc_fuel: nat) (fresh: MH.heap_chunk)
